Fix theory/chan except for select proof

new/golang/defn/chan.v
@@ -6,9 +6,9 @@ Section defns.
 Context {ext : ffi_syntax} {go_gctx : GoGlobalContext}.
 
 Definition receive elem_type : val :=
-  λ: "c", MethodResolve (channel.Channel elem_type) "Receive" #() "c".
+  λ: "c", MethodResolve (go.PointerType $ channel.Channel elem_type) "Receive" #() "c" #().
 Definition send elem_type : val :=
-  λ: "c", MethodResolve (channel.Channel elem_type) "Send" #() "c".
+  λ: "c", MethodResolve (go.PointerType $ channel.Channel elem_type) "Send" #() "c".
 
 Definition for_range elem_type : val :=
   λ: "c" "body",
@@ -79,13 +79,13 @@ Class ChanSemantics `{!GoSemanticsFunctions} :=
     (λ: "<>", FuncResolve go.make2 [elem_type] #() #(W64 0))%V;
   #[global] close_chan dir elem_type ::
     FuncUnfold go.close [go.ChannelType dir elem_type]
-    (λ: "c", MethodResolve (channel.Channel elem_type) "Close" #() "c")%V;
+    (λ: "c", MethodResolve (go.PointerType $ channel.Channel elem_type) "Close" #() "c" #())%V;
   #[global] len_chan dir elem_type ::
     FuncUnfold go.len [go.ChannelType dir elem_type]
-    (λ: "c", MethodResolve (channel.Channel elem_type) "Len" #() "c")%V;
+    (λ: "c", MethodResolve (go.PointerType $ channel.Channel elem_type) "Len" #() "c" #())%V;
   #[global] cap_chan dir elem_type ::
     FuncUnfold go.cap [go.ChannelType dir elem_type]
-    (λ: "c", MethodResolve (channel.Channel elem_type) "Cap" #() "c")%V;
+    (λ: "c", MethodResolve (go.PointerType $ channel.Channel elem_type) "Cap" #() "c" #())%V;
 
   chan_select_nonblocking default_handler clauses :
     is_go_step_pure SelectStmt (SelectStmtClausesV (Some default_handler) clauses) =
